src/tactic/nccc/backtrack.lean
@@ -1,0 +1,29 @@
+universes u v
+variables {α β : Type u}
+variable {m : Type u → Type v}
+variable [monad m]
+
+def monad.concat : list (m (list α)) → m (list α) 
+| []      := return []
+| (f::fs) :=
+  do l₁ ← f,
+     l₂ ← monad.concat fs, 
+     return (l₁ ++ l₂)
+
+@[reducible] def backtrack (m : Type u → Type v) := m ∘ list 
+
+namespace backtrack
+
+open list
+     
+@[inline] protected def pure (a : α) : backtrack m α := (return [a] : m (list α))
+
+@[inline] protected def bind (f : backtrack m α) 
+  (g : α → backtrack m β) : backtrack m β :=
+@bind m _ (list α) (list β) f (monad.concat ∘ (map g))
+
+instance monad : monad (backtrack m) :=
+{ pure := λ α, backtrack.pure, 
+  bind := λ α β, backtrack.bind }
+
+end backtrack
