src/tactic/nccc/backtrack_choice.lean
@@ -1,0 +1,39 @@
+universes u v w x
+variables {α : Type u}
+variables {β : Type u}
+variable {m : Type u → Type v}
+variables [monad m] [alternative m]
+
+inductive tree (α : Type u)
+| leaf : α → tree
+| fork : tree → tree → tree
+
+open tree 
+
+def tree.map {γ : Type w} {δ : Type x} (f : γ → δ) : tree γ → tree δ 
+| (leaf a)   := leaf (f a)
+| (fork t s) := fork t.map s.map 
+
+def flatten : tree (m (tree α)) → m (tree α) 
+| (leaf f)   := f
+| (fork f g) := 
+  do c ← flatten f, 
+     d ← flatten g, 
+     return (fork c d)
+
+@[reducible] def backtrack (m : Type u → Type v) := m ∘ tree 
+
+namespace backtrack
+     
+@[inline] protected def pure (a : α) : backtrack m α := 
+(return (leaf a) : m (tree α))
+
+@[inline] protected def bind (f : backtrack m α) 
+  (g : α → backtrack m β) : backtrack m β :=
+@bind m _ (tree α) (tree β) f (flatten ∘ (tree.map g))
+
+instance monad : monad (backtrack m) :=
+{ pure := λ α, backtrack.pure, 
+  bind := λ α β, backtrack.bind }
+
+end backtrack
