src/tactic/nccc/lit.lean
@@ -2,13 +2,16 @@ import .term
 
 variable {α : Type}
 
-@[derive has_reflect]
+@[derive has_reflect, derive decidable_eq]
 structure lit :=
 (sign : bool)
 (idx : nat)
 (args : list term)
 
 namespace lit
+
+def neg : lit → lit
+| ⟨b, k, ts⟩ := ⟨bnot b, k, ts⟩
 
 def holds (M : model α) (v : nat → α) : lit → Prop
 | ⟨tt, k, ts⟩  :=    M.rels k (ts.map (term.val M v))
@@ -23,5 +26,7 @@ instance has_repr : has_repr lit := ⟨repr⟩
 
 meta instance has_to_format : has_to_format lit := ⟨λ x, repr x⟩
 
+def vdxs : lit → list nat 
+| ⟨_, _, ts⟩ := ⋃ (ts.map term.vdxs)
 
 end lit
