src/tactic/nccc/mat.lean
@@ -1,0 +1,35 @@
+import .form
+
+local notation  `⊤*` := form.true
+local notation  `⊥*` := form.false
+local notation  `⟪` l `⟫` := form.lit l
+local notation  p `∨*` q := form.or p q
+local notation  p `∧*` q := form.and p q
+local notation  `∀*` := form.fa
+local notation  `∃*` := form.ex
+
+@[reducible] def mat : Type := list (list lit)
+
+namespace mat
+
+variable {α : Type}
+
+def holds (M : model α) (v : nat → α) (m : mat) : Prop :=
+∃ c ∈ m, ∀ l ∈ c, lit.holds M v l
+
+def valsat (α m) : Prop :=
+∀ M : model α, ∃ v : nat → α, (holds M v m)
+
+end mat
+
+def dnf : form → mat
+| ⊤*       := [[]]
+| ⊥*       := []
+| ⟪l⟫      := [[l]]
+| (p ∧* q) := (list.product (dnf p) (dnf q)).map (λ x, x.fst ++ x.snd)
+| (p ∨* q) := (dnf p) ++ (dnf q)
+| (∀* p)   := [] -- Irrelevant
+| (∃* p)   := [] -- Irrelevant
+
+lemma form_valsat_of_mat_valsat (α : Type) (p : form) :
+  p.quant_free → (dnf p).valsat α → p.valsat α := sorry
