src/tactic/nccc/misc.lean
@@ -9,4 +9,7 @@ def update_zero (a : α) (f : nat → α) : nat → α
 | 0     := a
 | (k+1) := f k
 
+meta def list_reflect [has_reflect α] (l : list α) : list expr :=
+l.map (λ x, `(x).to_expr)
+
 local notation f `₀↦` a := update_zero a f
