src/tactic/nccc/pnf.lean
@@ -1,0 +1,43 @@
+import .form
+
+
+local notation  `⊤*` := form.true
+local notation  `⊥*` := form.false
+local notation  `⟪` l `⟫` := form.lit l
+local notation  p `∧*` q := form.and p q
+local notation  p `∨*` q := form.or p q
+local notation  `∀*` := form.fa
+local notation  `∃*` := form.ex
+
+-- | ⊤*        := sorry
+-- | ⊥*        := sorry
+-- | ⟪⟨s, k, ts⟩⟫ := sorry
+-- | (p ∧* q)  := sorry
+-- | (p ∨* q)  := sorry
+-- | (∀* p)  := sorry
+-- | (∃* p)  := sorry
+
+def pnf_right (c : form → form → form) : form → form → form
+| p (∀* q) := ∀* (pnf_right (p.incr_vdx 0) q)
+| p (∃* q) := ∃* (pnf_right (p.incr_vdx 0) q)
+| p      q := c p q
+
+def pnf_left (c : form → form → form) : form → form → form
+| (∀* p) q := ∀* (pnf_left p (q.incr_vdx 0))
+| (∃* p) q := ∃* (pnf_left p (q.incr_vdx 0))
+| p      q := pnf_right c p q
+
+/- Assumes ∀-free input formulas -/
+def pnf : form → form
+| ⊤*       := ⊤*
+| ⊥*       := ⊥*
+| ⟪l⟫      := ⟪l⟫
+| (p ∨* q) := pnf_left (∨*) (pnf p) (pnf q)
+| (p ∧* q) := pnf_left (∧*) (pnf p) (pnf q)
+| (∀* p)   := ∀* (pnf p)
+| (∃* p)   := ∃* (pnf p)
+
+-- lemma valid_skolemize_core_imp (α : Type) (p : form) :
+
+lemma valid_pnf_imp (α : Type) (p : form) :
+  (pnf p).valid α → p.valid α := sorry
