src/tactic/nccc/proof.lean
@@ -1,0 +1,67 @@
+import .mat
+
+@[reducible] def cla : Type := list lit
+
+@[reducible] def sub : Type := list (nat × term)
+
+local notation  `#` := term.var
+local notation  `&` := term.fnc
+local notation  t1 `^*` t2 := term.app t1 t2
+
+def cla.is_pos (C : cla) : bool := C.all lit.sign
+
+def cla.vdxs (C : cla) : list nat := ⋃ (C.map lit.vdxs)
+
+def sub.term_app_aux (k : nat) : sub → term
+| []         := #k
+| ((m,t)::σ) :=
+  if k = m then t else sub.term_app_aux σ
+
+def sub.term_app (σ : sub) : term → term
+| (# k) := sub.term_app_aux k σ
+| (& k) := & k
+| (t ^* s) := (sub.term_app t) ^* (sub.term_app s)
+
+def sub.lit_app (σ : sub) : lit → lit
+| ⟨b, m, ts⟩ := ⟨b, m, ts.map σ.term_app⟩
+
+inductive proof : cla → mat → cla → Type
+| axm {M : mat} {P : cla} : proof [] M P
+| red {M : mat} {C P : cla} {L : lit} :
+  L.neg ∈ P → proof C M P → proof (L::C) M P
+| ext {M : mat} {C P : cla} {L : lit} (C₁ : cla) :
+  C₁ ∈ M → proof C M P →
+  proof (C₁.erase L.neg) (M.erase C₁) (L::P) →
+  proof (L::C) M P
+| cxt {M : mat} {C P : cla} (C₁ : cla) (L : lit) (σ : sub) :
+  C₁ ∈ M → proof C M P →
+  proof ((C₁.map (σ.lit_app)).erase L.neg) M (L::P) →
+  proof (L::C) M P
+
+
+
+
+#exit
+open expr tactic
+
+meta def foo : tactic unit :=
+do m ← tactic.mk_meta_var `(term),
+  trace m,
+  (unify m `(term.var 0) >> trace m >> failed) <|>
+  (trace m >> skip)
+
+example : false := by foo
+
+
+
+#exit
+
+def sub.term_app : sub → term → term
+| (# _)    := 0
+| (& n)    := n + 1
+| (t ^* s) := max (fresh_sdx t) (fresh_sdx s)
+
+
+def sub.lit_app (σ : sub) (l : lit) : lit :=
+
+#exit
