src/tactic/nccc/search.lean
@@ -1,0 +1,244 @@
+import .proof .misc
+
+universes u v
+variables {α β : Type}
+
+local notation  `#` := term.var
+local notation  `&` := term.fnc
+local notation  t `^*` s := term.app t s
+
+meta def clax : Type := list expr
+meta def subx : Type := list (nat × expr)
+
+@[reducible] meta def goal : Type := clax × mat × clax
+
+meta def goal.to_format : goal → format 
+| ⟨Cx, M, Px⟩ := 
+  "(Clause : " ++ Cx.to_format ++ ", Matrix : " ++ M.to_format ++ 
+  ", Path : " ++ Px.to_format ++ ")"
+
+meta instance goal.has_to_format : has_to_format goal := ⟨goal.to_format⟩ 
+
+meta inductive rule : Type
+| start : nat → option subx → rule
+| red   : nat → rule
+| ext   : nat → nat → option subx → rule 
+
+meta def rule.to_format : rule → format 
+| (rule.start k σ) := "Start " ++ k.repr ++ " _"
+| (rule.red k )    := "Reduction " ++ k.repr 
+| (rule.ext k m σ) := "Extend " ++ k.repr ++ " " ++ m.repr ++ " _"
+
+meta instance rule.has_to_format : has_to_format rule := ⟨rule.to_format⟩ 
+
+meta structure search_state :=
+(max : nat)
+(lim : nat)
+(goals : list goal)
+(rules : list rule)
+
+meta def search_state.to_format : search_state → format 
+| ⟨m, l, gs, rs⟩ := 
+  "Max : " ++ m.repr ++ "\n" ++
+  "Lim : " ++ l.repr ++ "\n" ++
+  "Goals : " ++ gs.to_format ++ "\n" ++ 
+  "Rules : " ++ rs.to_format ++ "\n" 
+
+meta instance search_state.has_to_format : has_to_format search_state := 
+⟨search_state.to_format⟩ 
+
+@[reducible] meta def search := state_t search_state tactic
+
+meta def get_max : search nat := search_state.max <$> get
+meta def get_lim : search nat := search_state.lim <$> get
+meta def get_goals : search (list goal) := search_state.goals <$> get
+meta def get_rules : search (list rule) := search_state.rules <$> get
+
+meta def set_max (m : nat) : search unit := modify $ λ s, {max := m, .. s}
+meta def set_lim (l : nat) : search unit := 
+--state_t.lift (tactic.trace "Setting lim to : " >> tactic.trace l) >>
+(modify $ λ s, {lim := l, .. s})
+meta def set_goals (gs : list goal) : search unit := modify $ λ s, {goals := gs, .. s}
+meta def set_rules (rs : list rule) : search unit := modify $ λ s, {rules := rs, .. s}
+
+meta def pop_goal : search goal := 
+do (g::gs) ← get_goals,
+   set_goals gs,
+   return g
+
+meta def print [has_to_tactic_format α] (a : α) : search unit :=
+state_t.lift (tactic.trace a)
+
+meta def push_goal (g : goal) : search unit := 
+do gs ← get_goals,
+   set_goals (g::gs)
+   
+
+meta def push_rule (r : rule) : search unit := 
+do rs ← get_rules,
+   set_rules (r::rs)
+
+meta def failed {α : Type} : search α := ⟨λ x, tactic.failed⟩
+
+meta def skip : search unit := ⟨λ x, return ⟨(), x⟩⟩  
+
+meta def backtrack (α : Type) : Type := (nat → search α) × nat
+
+@[reducible] meta def bsearch (α : Type) : Type := search (backtrack α) 
+
+meta def bbind_core : backtrack α → (α → search β) → search β 
+| (s, 0)     t := failed
+| (s, k + 1) t := (s k >>= t) <|> (bbind_core (s, k) t)
+
+meta def bbind (b : bsearch α) (s : α → search β) : search β :=
+b >>= λ x, bbind_core x s
+infixr `>>>=` : 1100 := bbind 
+
+meta def bthen (b : bsearch α) (s : search β) : search β :=
+b >>>= (λ _, s)
+
+infixr `>>>` : 1100 := bthen
+
+meta def pick_lim : search (backtrack unit) := 
+do m ← get_max,
+   l ← get_lim,
+   return (λ x, set_lim (m - x), (m - l) + 1) 
+
+meta def subx.mk : list nat → tactic subx 
+| []      := return []
+| (k::ks) := 
+  do sx ← subx.mk ks,
+     tx ← tactic.mk_meta_var `(term),
+     return ((k,tx)::sx)
+
+meta def subx.subst (k : nat) : subx → expr 
+| []          := `(# k)
+| ((m,tx)::σ) := 
+  if k = m then tx else subx.subst σ 
+
+meta def termx.mk (σ : subx) : term → expr 
+| (# k)    := subx.subst k σ  
+| (& k)    := `(& k)
+| (t ^* s) := `(%%(termx.mk t) ^* %%(termx.mk s))
+
+meta def termsx.mk (σ : subx) : list term → expr 
+| []      := `(@list.nil term)
+| (t::ts) := `(@list.cons term %%(termx.mk σ t) %%(termsx.mk ts))
+
+meta def litx.mk (σ : subx) : lit → expr 
+| ⟨b, k, ts⟩ := `(lit.mk %%`(b) %%`(k) %%(termsx.mk σ ts))
+
+meta def pick_cla_aux (M : mat) (k : nat) : search unit := 
+match M.nth k with 
+| none   := failed
+| some C := 
+  if cla.is_pos C
+  then match cla.vdxs C with
+       | []        := 
+         do push_goal (C.map (litx.mk []), M.erase C, []),
+            push_rule (rule.start k none) 
+       | vs@(_::_) := 
+         do σ ← state_t.lift (subx.mk vs), 
+            push_goal ⟨C.map (litx.mk σ), M, []⟩,
+            push_rule (rule.start k σ) 
+       end
+  else failed
+end
+
+meta def pick_cla : search (backtrack unit) := 
+do (_, M, _) ← pop_goal, 
+   return (pick_cla_aux M, M.length)
+
+meta def negx.mk : expr → search expr 
+| `(lit.mk %%bx %%kx %% tsx) := 
+  return `(lit.mk (bnot %%bx) %%kx %% tsx) 
+| _ := failed
+
+meta def comp_unify (L N : expr): search unit := 
+do negL ← negx.mk L,
+   state_t.lift (tactic.unify N negL)
+
+meta def reduce_aux (L : expr) (M : mat) (C P : clax) (k : nat) : search unit :=
+match P.nth k with 
+| none := failed
+| some N := 
+  do comp_unify L N,
+     push_goal (C,M,P)
+end
+
+meta def reduce : bsearch unit := 
+( ( do 
+  ⟨L::C, M, P⟩ ← pop_goal,
+  return (reduce_aux L M C P, P.length) ) 
+  : search (backtrack unit) )
+
+def maxlen (l : list (list α)) : nat :=
+(l.map list.length).max
+
+def mat.entry (M : mat) (i j : nat) : option lit := 
+do C ← M.nth j, C.nth i
+
+meta def option.to_search : option α → search α 
+| none     := failed
+| (some a) := return a
+
+meta def extend_aux (Lx : expr) (M : mat) (Cx Px : clax) (km : nat) : search unit := 
+let i : nat := km % maxlen M in 
+let j : nat := km / maxlen M in 
+do D ← (M.nth j).to_search,
+   match cla.vdxs D with 
+   | [] :=
+     let Dx := D.map (litx.mk []) in
+     do Nx ← (Dx.nth i).to_search,
+        comp_unify Lx Nx,
+        push_goal (Dx.except i, M.except j, Lx::Px),
+        push_goal (Cx, M, Px),
+        push_rule (rule.ext j i none)
+   | vs@(_::_) := 
+     do σ ← state_t.lift (subx.mk vs), 
+        Dx ← return (D.map (litx.mk σ)),
+        Nx ← (Dx.nth i).to_search,
+        comp_unify Lx Nx,
+        push_goal (Dx.except i, M, Lx::Px),
+        push_goal (Cx, M, Px),
+        push_rule (rule.ext j i σ)
+   end
+
+meta def extend : bsearch unit :=  
+( ( do 
+  l ← get_lim,
+  (Lx::Cx, M, Px) ← pop_goal,
+  if Px.length < l
+  then return (extend_aux Lx M Cx Px, M.length * maxlen M)  
+  else failed )
+  : search (backtrack unit) )
+
+meta def close : search unit := 
+do ⟨[], _, _⟩ ← pop_goal, skip
+
+meta def finish : search unit := 
+do gs ← get_goals, 
+   if gs = [] then skip else failed
+
+local attribute [inline] state_t.orelse
+
+meta def loop : search unit :=
+--do print "Current goals : ", 
+--   get_goals >>= print,
+( (reduce >>> loop) <|> (extend >>> loop) <|>
+  (close >> loop) <|> finish )
+
+meta def main : search unit := 
+pick_lim >>> pick_cla >>> loop 
+
+meta def mk_search_state (M : mat) (l : nat := M.length)
+  (m : nat := l * 2) : tactic search_state :=
+return ⟨m, l, [⟨[], M, []⟩], []⟩ 
+
+meta def derive (M : mat) : tactic (list rule) := 
+(list.reverse ∘ search_state.rules) <$> prod.snd <$> 
+  (mk_search_state M >>= @state_t.run search_state tactic unit main)
+
+def socrates : mat := [[⟨tt, 0, [& 0]⟩, ⟨tt, 1, [& 1]⟩], [⟨ff, 0, [& 0]⟩], [⟨ff, 1, [& 1]⟩]]
+
+run_cmd derive socrates >>= tactic.trace
